\documentclass{article}
\usepackage{amsmath}
\usepackage{amssymb}
\begin{document}

Here I will derive the \textbf{Fast Fourier Transform} from the Discrete Fourier transform equation given by wikipedia using the same symmetry exploited by the \textbf{Cooleyâ€“Tukey} algorithm. \\ \\
Lets begin... \\
%
Start with the general Fourier transform equation...
$$X_k = \sum_{n=0}^{N-1}x_n(cos(-2\pi k \frac{n}{N}) + i sin(-2\pi k \frac{n}{N})), k \in \mathbb{Z}$$
We will apply euler's identity $e^{ix} = cos(x) + i sin(x)$ \\
$$X_k = \sum_{n=0}^{N-1}x_n \cdot e^{-i2\pi k \frac{n}{N}}, k \in \mathbb{Z}$$
This form makes the equation simpler for optimizatin shown below \\

\begin{align*}
X_k &= \sum_{n=0}^{N-1}x_n \cdot e^{-i2\pi k \frac{n}{N}} \\
&= \sum_{m=0}^{N/2-1}x_{2m} \cdot e^{-i2\pi k \frac{2m}{N}} + \sum_{m=0}^{N/2-1}x_{2m+1} \cdot e^{-i2\pi k \frac{2m+1}{N}} \\
&= (\sum_{m=0}^{N/2-1}x_{2m} \cdot e^{-i2\pi k \frac{2m}{N}}) + e^{-i2\pi k \frac{1}{N}} \sum_{m=0}^{N/2-1}x_{2m+1} \cdot e^{-i2\pi k \frac{2m}{N}} \\
\end{align*}

\end{document}w